@prefix rdf: <http://www.w3.org/1999/02/22-rdf-syntax-ns#> .
@prefix rdfs: <http://www.w3.org/2000/01/rdf-schema#> .
@prefix xml: <http://www.w3.org/XML/1998/namespace> .
@prefix owl:  <http://www.w3.org/2002/07/owl#> .
@prefix therapy: <https://schema.org/MedicalTherapy#>
@prefix drug: <https://schema.org/Drug#>
@prefix symptom: <https://schema.org/MedicalSignOrSymptom#>
@prefix test: <https://schema.org/MedicalTest#>
@prefix : <https://schema.org/MedicalCondition#>


# Declaration of the Ontology
: a owl:Ontology ;
    rdfs:label "Toy Medical Condition Ontology" ;
    rdfs:comment "An example schema to describe medical case reports." .

# Define Classes
# The medical condition of a patient
:medicalCondition a rdfs:Class ;
    rdfs:label "MedicalCondition" ;
    rdfs:comment "Any condition of the human body that affects the normal functioning of a person." .

# A patient typically has some signs or symptoms of his medical condition
symptom:medicalSignOrSymptom a rdfs:Class ;
    rdfs:label "MedicalSignOrSymptom" ;
    rdfs:comment "Any feature associated or not with a medical condition. In medicine a symptom is generally subjective while a sign is objective." .

# The medical therapy given to the patient after the examination
therapy:medicalTherapy a rdfs:Class ;
    rdfs:label "MedicalTherapy" ;
    rdfs:comment "Any medical intervention designed to prevent, treat, and cure human diseases." .

# The medical therapy can include some drugs
drug:drug a rdfs:Class ;
    rdfs:label "Drug" ;
    rdfs:comment "A chemical or biologic substance, used as a medical therapy, that has a physiological effect on an organism." .

# The test done to define the medical condition of a patient (there can be many)
test:medicalTest a rdfs:Class ;
    rdfs:label "MedicalTest" ;
    rdfs:comment "Any medical test, typically performed for diagnostic purposes." .

# Define Properties
test:hasMedicalCondition a rdf:Property ;
    rdfs:label "hasMedicalCondition" ;
    rdfs:comment "A medical condition determined after the test" ;
    rdfs:domain test:medicalTest ;
    rdfs:range :medicalCondition .

test:testType a rdf:Property ; #text
    rdfs:label "testType" ;
    rdfs:comment "A type of test performed to identify the medical condition of a patient e.g.'palpation'." ;
    rdfs:domain test:medicalTest .

:hasSignOrSymptom a rdf:Property ;
    rdfs:label "hasSignOrSymptom" ;
    rdfs:comment "A sign or symptom of this condition. Signs are objective or physically observable manifestations of the medical condition while symptoms are the subjective experience of the medical condition." ;
    rdfs:domain :medicalCondition ;
    rdfs:range symptom:medicalSignOrSymptom .

symptom:signOrSymptomName a rdf:Property ; #text
    rdfs:label "signOrSymptomName"
    rdfs:comment "The name of a sign or a symptom e.g. 'fever'." ;
    rdfs:domain symptom:medicalSignOrSymptom .

:hasMedicalTherapy a rdf:Property ;
    rdfs:label "hasMedicalTherapy" ;
    rdfs:comment "The medical therapy of the medical condition of the patient." ;
    rdfs:domain :medicalCondition ;
    rdfs:range therapy:medicalTherapy .

therapy:hasFollowup a rdf:Property ; #text
    rdfs:label "hasFollowup" ;
    rdfs:comment "Typical or recommended follow-up care after the procedure is performed." ;
    rdfs:domain therapy:medicalTherapy .

therapy:hasDrug a rdf:Property ;
    rdfs:label "hasDrug" ;
    rdfs:comment "Specifies a drug or medicine used in a medication procedure." ;
    rdfs:domain therapy:medicalTherapy ;
    rdfs:range drug:Drug .

drug:activeIngredient a rdf:Property ; #text
    rdfs:label "activeIngredient" ;
    rdfs:comment "An active ingredient, typically chemical compounds and/or biologic substances." ;
    rdfs:domain drug:Drug .

drug:administrationRoute a rdf:Property ; #text
    rdfs:label "administrationRoute" ;
    rdfs:comment "A route by which this drug may be administered, e.g. 'oral'." ;
    rdfs:domain drug:Drug .


"""
- Medical test : done
- symptoms or signs, : done
- diagnosis, : done
+ additional examination : another medical test
- treatment / drug, : done
- follow-up : done

- effectiveness : optional
- adverse events : optional (associated to the medical therapy)
"""